src/DiskSecAttacker.v
@@ -416,3 +416,283 @@ Proof.
     eapply XRCrashedRecovered; eauto.
   }
 Qed.
+
+
+  Lemma exec_equivalent_for_viewer_finished:
+  forall T (p: prog T) caller viewer d d' bm bm' hm d1 bm1 hm1 r1 tr,
+    exec caller d bm hm p (Finished d1 bm1 hm1 r1) tr ->
+    (forall tag, can_access viewer tag -> equivalent_for tag d d') ->
+    (forall tag, can_access viewer tag -> blockmem_equivalent_for tag bm bm') ->
+    only_public_operations tr ->
+    exists d2 bm2 tr2,
+      exec caller d' bm' hm p (Finished d2 bm2 hm1 r1) tr2 /\
+      (forall tag, can_access viewer tag -> equivalent_for tag d1 d2) /\
+      (forall tag, can_access viewer tag -> blockmem_equivalent_for tag bm1 bm2).
+  Proof.
+     induction p; intros;  
+  inv_exec_perm; cleanup; simpl in *;
+  try solve [repeat eexists; [econstructor; eauto|eauto|eauto] ].
+  { (** Read **)
+    destruct tb.
+    specialize H1 with (1:= can_access_public viewer) as Hx;
+    specialize (Hx r1); intuition; cleanup; try congruence.
+    specialize H0 with (1:= can_access_public viewer) as Hx;
+    specialize (Hx n); intuition; cleanup; try congruence.
+    destruct x0, t0.
+    unfold vsmerge in *; simpl in *.
+    inversion H5; inversion H6; simpl in *; subst.
+    do 3 eexists; split.
+    econstructor; eauto.
+    split; eauto.
+    unfold blockmem_equivalent_for; intros.
+    destruct (handle_eq_dec a r1); subst.
+    right.
+    repeat rewrite Mem.upd_eq; eauto.
+    do 2 eexists; eauto.
+    split; eauto.
+    split; eauto.
+    split; eauto.
+    intros.
+    simpl in *; eauto.    
+    specialize H0 with (1:= H) as Hx;
+    specialize (Hx n); intuition; cleanup; try congruence.
+    unfold vsmerge in *; simpl in *.
+    inversion H10; inversion H12; simpl in *; subst.
+    eauto.
+    repeat rewrite Mem.upd_ne; eauto.
+    eapply H1; eauto.
+  }
+  { (** Write **)
+    destruct tb, tbs, t0.
+    destruct (can_access_dec viewer t).
+    { (** can access **)
+      specialize H0 with (1:= can_access_public viewer) as Hx;
+      specialize (Hx n); intuition; cleanup; try congruence.
+      specialize H1 with (1:= c) as Hx;
+      specialize (Hx h); intuition; cleanup; try congruence.
+      destruct x0, x1; simpl in *; cleanup.
+      do 3 eexists; split.
+      econstructor; eauto.
+      split; eauto.
+      unfold equivalent_for; intros.
+      specialize H0 with (1:= H) as Hx;
+      specialize (Hx n); destruct Hx; cleanup; try congruence.
+      destruct (addr_eq_dec a n); subst.
+      right.
+      repeat rewrite Mem.upd_eq; eauto.
+      do 2 eexists; eauto.
+      split; eauto.
+      split; eauto.
+      split.
+      unfold vsmerge in *; simpl in *; eauto.
+      unfold vsmerge in *; simpl in *; eauto.
+      repeat rewrite Mem.upd_ne; eauto.
+      eapply H0; eauto.
+    }
+    { (** can't access **)
+      specialize H0 with (1:= can_access_public viewer) as Hx;
+      specialize (Hx n); intuition; cleanup; try congruence.
+      specialize H1 with (1:= can_access_public viewer) as Hx;
+      specialize (Hx h); intuition; cleanup; try congruence.
+      destruct x0, x1; simpl in *; cleanup.
+      do 3 eexists; split.
+      econstructor; eauto.
+      split; eauto.
+      unfold equivalent_for; intros.
+      destruct (tag_dec t2 tag); subst; intuition.
+      specialize H0 with (1:= H) as Hx;
+      specialize (Hx n); destruct Hx; cleanup; try congruence.
+      destruct (addr_eq_dec a n); subst.
+      right.
+      repeat rewrite Mem.upd_eq; eauto.
+      do 2 eexists; eauto.
+      split; eauto.
+      split; eauto.
+      split.
+      unfold vsmerge in *; simpl in *; eauto.
+      unfold vsmerge in *; simpl in *; eauto.
+      econstructor.
+      simpl; intros; intuition.
+      eauto.
+      repeat rewrite Mem.upd_ne; eauto.
+      eapply H0; eauto.
+    }
+  }
+  { (** Seal **)
+    specialize H1 with (1:= can_access_public viewer) as Hx;
+    specialize (Hx r1); intuition; cleanup; try congruence.
+    do 3 eexists; split.
+    econstructor; eauto.
+    split; eauto.
+    unfold blockmem_equivalent_for; intros.
+    destruct (handle_eq_dec a r1); subst.
+    right.
+    repeat rewrite Mem.upd_eq; eauto.
+    do 2 eexists; eauto.
+    repeat rewrite Mem.upd_ne; eauto.
+    eapply H1; eauto.
+  }
+  { (** Unseal **)
+    intuition.
+    destruct tb; simpl in *.
+    specialize H1 with (1:= can_access_public viewer) as Hx;
+    specialize (Hx h); intuition; cleanup; try congruence.
+    simpl in *; intuition; subst.
+    do 3 eexists; split.
+    econstructor; eauto.
+    split; eauto.
+  }
+  { (** Sync **)
+    repeat eexists; [econstructor; eauto| |eauto].
+    unfold equivalent_for in *; intros.
+    specialize H0 with (1:= H) as Hx.
+    unfold sync_mem.
+    specialize (Hx a); intuition; cleanup; eauto.
+    rewrite H4, H5; eauto.
+    rewrite H3, H4; eauto.
+    destruct x, x0.
+    right; repeat eexists; eauto.
+    unfold vsmerge in *; simpl in *; eauto.
+    inversion H5; subst.
+    econstructor; eauto.
+    unfold vsmerge in *; simpl in *; eauto.
+    inversion H6; subst; auto.
+  }
+  { (** Bind **)
+    apply only_public_operations_app in H3; cleanup.
+    specialize IHp with (1:=H0)(2:=H1)(3:=H2)(4:=H5); cleanup.
+    specialize H with (1:=H4)(2:=H7)(3:=H8)(4:=H3); cleanup.
+    repeat eexists; [econstructor; eauto| |]; eauto.
+  }
+  Qed.
+
+  Lemma exec_equivalent_for_viewer_failed:
+  forall T (p: prog T) caller viewer d d' bm bm' hm d1 bm1 hm1 tr,
+    exec caller d bm hm p (Failed d1 bm1 hm1) tr ->
+    (forall tag, can_access viewer tag -> equivalent_for tag d d') ->
+    (forall tag, can_access viewer tag -> blockmem_equivalent_for tag bm bm') ->
+    only_public_operations tr ->
+    exists d2 bm2 tr2,
+      exec caller d' bm' hm p (Failed d2 bm2 hm1) tr2 /\
+      (forall tag, can_access viewer tag -> equivalent_for tag d1 d2) /\
+      (forall tag, can_access viewer tag -> blockmem_equivalent_for tag bm1 bm2).
+  Proof.
+  induction p; intros;  
+  inv_exec_perm; cleanup; simpl in *;
+  try solve [repeat eexists; [econstructor; eauto|eauto|eauto] ].
+  { (** Read **)
+    specialize H0 with (1:= can_access_public viewer) as Hx;
+    specialize (Hx n); intuition; cleanup; try congruence.
+    do 3 eexists; split.
+    econstructor; eauto.
+    split; eauto.
+  }
+  { (** Write **)
+    intuition.
+    { (** bm1 h = None **)
+      specialize H1 with (1:= can_access_public viewer) as Hx;
+      specialize (Hx h); intuition; cleanup; try congruence.
+      do 3 eexists; split.
+      econstructor; eauto.
+      split; eauto.
+    }
+    { (** d1 n = None **)
+      specialize H0 with (1:= can_access_public viewer) as Hx;
+      specialize (Hx n); intuition; cleanup; try congruence.
+      do 3 eexists; split.
+      econstructor; eauto.
+      split; eauto.
+    }
+  }
+  { (** Unseal **)
+    specialize H1 with (1:= can_access_public viewer) as Hx;
+    specialize (Hx h); intuition; cleanup; try congruence.
+    do 3 eexists; split.
+    econstructor; eauto.
+    split; eauto.
+  }
+  { (** Bind **)
+    intuition.
+    { (** p Failed **)
+      specialize IHp with (1:=H4)(2:=H1)(3:=H2)(4:=H3); cleanup.
+      do 3 eexists; split.
+      eapply FailBind; eauto.
+      eauto.
+    }
+    { (** p0 Failed **)
+      cleanup.
+      apply only_public_operations_app in H3; cleanup.
+      eapply exec_equivalent_for_viewer_finished in H0; eauto; cleanup.
+      specialize H with (1:=H4)(2:=H6)(3:=H7)(4:=H3); cleanup.
+      do 3 eexists; split.
+      econstructor; eauto.
+      eauto.
+    }
+  }
+  Qed.
+
+  Lemma exec_equivalent_for_viewer_crashed:
+  forall T (p: prog T) caller viewer d d' bm bm' hm d1 bm1 hm1 tr,
+    exec caller d bm hm p (Crashed d1 bm1 hm1) tr ->
+    (forall tag, can_access viewer tag -> equivalent_for tag d d') ->
+    (forall tag, can_access viewer tag -> blockmem_equivalent_for tag bm bm') ->
+    only_public_operations tr ->
+    exists d2 bm2 tr2,
+      exec caller d' bm' hm p (Crashed d2 bm2 hm1) tr2 /\
+      (forall tag, can_access viewer tag -> equivalent_for tag d1 d2) /\
+      (forall tag, can_access viewer tag -> blockmem_equivalent_for tag bm1 bm2).
+  Proof.
+  induction p; intros;  
+  inv_exec_perm; cleanup; simpl in *;
+  try solve [repeat eexists; [econstructor; eauto|eauto|eauto] ].
+  { (** Bind **)
+    intuition.
+    { (** p Crashed **)
+      specialize IHp with (1:=H4)(2:=H1)(3:=H2)(4:=H3); cleanup.
+      do 3 eexists; split.
+      eapply CrashBind; eauto.
+      eauto.
+    }
+    { (** p0 crashed **)
+      cleanup.
+      apply only_public_operations_app in H3; cleanup.
+      eapply exec_equivalent_for_viewer_finished in H0; eauto; cleanup.
+      specialize H with (1:=H4)(2:=H6)(3:=H7)(4:=H3); cleanup.
+      do 3 eexists; split.
+      econstructor; eauto.
+      eauto.
+    }
+  }
+Qed.
+
+
+Lemma exec_equivalent_for_viewer:
+  forall T (p: prog T) caller viewer d d' bm bm' hm res tr,
+    exec caller d bm hm p res tr ->
+    (forall tag, can_access viewer tag -> equivalent_for tag d d') ->
+    (forall tag, can_access viewer tag -> blockmem_equivalent_for tag bm bm') ->
+    only_public_operations tr ->
+     (exists d1 bm1 hm1 r1, res = Finished d1 bm1 hm1 r1 /\ 
+      exists d2 bm2 tr2, exec caller d' bm' hm p (Finished d2 bm2 hm1 r1) tr2 /\
+      (forall tag, can_access viewer tag -> equivalent_for tag d1 d2) /\
+      (forall tag, can_access viewer tag -> blockmem_equivalent_for tag bm1 bm2)) \/
+      
+      (exists d1 bm1 hm1, res = Crashed d1 bm1 hm1 /\
+       exists d2 bm2 tr2, exec caller d' bm' hm p (Crashed d2 bm2 hm1) tr2 /\
+      (forall tag, can_access viewer tag -> equivalent_for tag d1 d2) /\
+      (forall tag, can_access viewer tag -> blockmem_equivalent_for tag bm1 bm2)) \/
+      
+      (exists d1 bm1 hm1, res = Failed d1 bm1 hm1 /\
+       exists d2 bm2 tr2, exec caller d' bm' hm p (Failed d2 bm2 hm1) tr2 /\
+      (forall tag, can_access viewer tag -> equivalent_for tag d1 d2) /\
+      (forall tag, can_access viewer tag -> blockmem_equivalent_for tag bm1 bm2)).
+Proof.
+  intros.
+  destruct res.
+  left; do 4 eexists; split; eauto.
+  eapply exec_equivalent_for_viewer_finished; eauto.
+  right; left; do 3 eexists; split; eauto.
+  eapply exec_equivalent_for_viewer_crashed; eauto.
+  right; right; do 3 eexists; split; eauto.
+  eapply exec_equivalent_for_viewer_failed; eauto.
+Qed.
